Starts JSML -> BFN translation. Del is kind of... broken.

bfn.v
@@ -15,8 +15,10 @@ Module BFN.
   | bfn_dec : nat -> BFN -> BFN   (* - *)
   | bfn_out : nat -> BFN -> BFN   (* . *)
   | bfn_in : nat -> BFN -> BFN    (* , *)
-  | bfn_loop : BFN -> BFN -> BFN.  (* [...] *)
-
+  | bfn_loop : BFN -> BFN -> BFN  (* [...] *)
+  | label : string -> BFN -> BFN
+  | assert : (nat -> bool) -> string -> BFN -> BFN.
+  
   Inductive BFNState : Type :=
     | running (ast: BFN)
               (resets: list BFN)
@@ -24,7 +26,8 @@ Module BFN.
               (tape: BFTape.Tape)
               (input: list nat)
               (output: list nat)
-    | halted (output: list nat).
+    | halted (output: list nat)
+    | error (msg: string).
 
   Function bfn_weight (bfn: BFN): nat :=
     match bfn with
@@ -36,17 +39,19 @@ Module BFN.
     | bfn_out n bfn'
     | bfn_in n bfn' => (S n) + bfn_weight bfn'
     | bfn_loop inner bfn' => S ((bfn_weight inner) + (bfn_weight bfn'))
+    | label string bfn' => S (bfn_weight bfn')
+    | assert b string bfn' => S (bfn_weight bfn')
     end.
 
   Function bfn_state_weight (s: BFNState): nat :=
     match s with
     | running bfn _ _ _ _ _ => bfn_weight bfn
-    | halted _ => 0
+    | halted _ | error _ => 0
     end.
 
   Function bfn_step (s: BFNState) {measure bfn_state_weight s}: BFNState :=
     match s with
-    | halted _ => s
+    | halted _ | error _ => s
     | running bfn resets ptr tape input output =>
       match bfn with
       | bfn_end =>
@@ -86,24 +91,137 @@ Module BFN.
           running bfn' resets ptr tape input output
         else
           running inner_bfn (bfn :: resets) ptr tape input output
+      | label str bfn' => running bfn' resets ptr tape input output
+      | assert truth msg bfn' => match truth ptr with
+         | true => running bfn' resets ptr tape input output
+         | false => error msg
+         end
       end
     end.
   Proof.
     all: intros; auto; simpl; omega.
-  Qed.
+  Defined.
 
   Function exec_init (prog: BFN) (input: list nat): BFNState :=
     running prog [] 0 BFTape.empty input [].
+
+Definition debug_bfn (prog: BFN) (input: list nat) (fuel: nat) :=
+    Utils.run bfn_step (exec_init prog input) fuel.
+    
 
   Definition interpret_bfn (prog: BFN) (input: list nat) (fuel: nat): option (list nat) :=
     match Utils.run bfn_step (exec_init prog input) fuel with
     | running _ _ _ _ _ _ => None
     | halted output => Some output
+    | error msg => None
     end.
 
+  Function bfn_append bfn1 bfn2 :=
+    match bfn1 with
+    | bfn_end => bfn2
+    | bfn_right n bfn' => bfn_right n (bfn_append bfn' bfn2)
+    | bfn_left n bfn' => bfn_left n (bfn_append bfn' bfn2)
+    | bfn_inc n bfn' => bfn_inc n (bfn_append bfn' bfn2)
+    | bfn_dec n bfn' => bfn_dec n (bfn_append bfn' bfn2)
+    | bfn_out n bfn' => bfn_out n (bfn_append bfn' bfn2)
+    | bfn_in n bfn' => bfn_in n (bfn_append bfn' bfn2)
+    | bfn_loop inner bfn' => bfn_loop inner (bfn_append bfn' bfn2)
+    | label str bfn' => label str (bfn_append bfn' bfn2)
+    | assert truth str bfn' => assert truth str (bfn_append bfn' bfn2)
+    end.
+
+  Notation "a & f" := (bfn_append a f) (at level 50, left associativity).
+  
+  Fixpoint repeat (n : nat) (bfn : BFN) : BFN :=
+    match n with
+    | 0 => bfn_end
+    | S m => bfn & repeat m bfn
+    end.
+  
+  Definition prev :=
+    label "prev" (bfn_left 3 (bfn_loop (bfn_left 3 bfn_end) bfn_end)).
+    
+  Definition next :=
+    label "next" (bfn_right 3 (bfn_loop (bfn_right 3 bfn_end) bfn_end)).
+    
+  Definition zero_cell :=
+    label "zero_cell" (bfn_loop (bfn_dec 1 bfn_end) bfn_end).
+    
+  Definition scc_right :=
+    label "scc_right" zero_cell & (bfn_right 1 (bfn_loop (bfn_dec 1 (bfn_left 1 (bfn_inc 1 (bfn_right 1 (bfn_end))))) 
+    (bfn_left 1 bfn_end))).
+  
+  Definition scc_left :=
+    label "scc_left" zero_cell & (bfn_left 1 (bfn_loop (bfn_dec 1 (bfn_right 1 (bfn_inc 1 (bfn_left 1 bfn_end)))) 
+    (bfn_right 1 bfn_end))).
+    
+  Definition skk := 
+    label "skk" zero_cell & (bfn_right 1 zero_cell) & (bfn_right 1 scc_right) & 
+    (bfn_loop (bfn_dec 1 (bfn_right 1 (bfn_inc 1 (bfn_left 3 (bfn_inc 1 (bfn_right 2 bfn_end)))))) 
+      ((bfn_right 3 scc_left) & 
+    (bfn_loop (bfn_dec 1 (bfn_left 1 (bfn_inc 1 (bfn_left 3 (bfn_inc 1 (bfn_right 4 bfn_end)))))) 
+      (bfn_left 5 bfn_end)))).
+      
+  Definition sik :=
+    label "sik" (skk & (bfn_right 6 (bfn_loop ((bfn_left 3 skk) & bfn_right 6 bfn_end) (bfn_left 3 prev)))).
+
+  Definition shift_item :=
+    label "shift_item" next & (bfn_left 3 (bfn_loop (sik & bfn_left 3 bfn_end) sik)).
+    
+  Definition zero_item :=
+    label "zero_item" (bfn_right 2 (zero_cell & (bfn_right 1 zero_cell) & (bfn_left 3 bfn_end))).
+
   (* JSML -> BFN. Stub. *)
-  Function bfn_of_jsm (jsm : JSML.JSMProgram * list JSML.JSMProgram) :=
-    let (main, fn_table) := jsm in
-    main.
+  Function bfn_of_jsm (main : JSML.JSMProgram) :=
+    match main with
+    | JSML.push n :: jsmp =>
+      let bfn := bfn_of_jsm jsmp in
+       (bfn_right 3 (bfn_inc 1 (bfn_right 1 (bfn_inc n (bfn_right 2 bfn))))) (* need to zero? *)
+    | JSML.del n :: jsmp =>
+      let bfn := bfn_of_jsm jsmp in
+      label "del" (repeat (n+1) prev) & (repeat n (shift_item & next)) & zero_item & bfn
+    | JSML.out :: jsmp =>
+      bfn_left 2 (bfn_out 1 (bfn_right 2 (bfn_of_jsm jsmp)))
+    | _ => bfn_end
+    end.
+  
+  Example bfn_of_jsml_push :
+    interpret_bfn (bfn_of_jsm [JSML.push 20; JSML.push 10; JSML.out]) [] 60 = Some [10].
+  Proof. auto. Qed.
+  
+  Example bfn_of_jsm1_del_0 :
+    interpret_bfn (bfn_of_jsm [JSML.push 10; JSML.push 20; JSML.del 0; JSML.out]) [] 700 = Some [10].
+  Proof. auto. Qed.
+  
+  
+  Example bfn_of_jsm1_del_1 :
+    interpret_bfn (bfn_of_jsm [JSML.push 10; JSML.push 20; JSML.del 1; JSML.out]) [] 1700 = Some [20].
+  Proof. auto. Qed. 
+  
+  
+  Example bfn_of_jsm1_del_1 :
+    interpret_bfn (bfn_of_jsm [JSML.push 10; JSML.push 20; JSML.del 1; JSML.out]) [] 1700 = Some [20].
+  Proof. auto. Qed.
+ 
+ 
+  
+  Eval compute in debug_bfn (bfn_of_jsm [JSML.push 5; JSML.push 2; JSML.push 3; JSML.del 1; JSML.out]) [] 2000.
+  
+ 
+  Eval compute in debug_bfn (bfn_of_jsm [JSML.push 5; JSML.push 2; JSML.push 3; JSML.del 2; JSML.out]) [] 350.
+ 
+  
+  Eval compute in debug_bfn (bfn_of_jsm [JSML.push 1; JSML.push 2; JSML.del 1; JSML.out]) [] .
+  
+  
+  Eval compute in bfn_of_jsm [JSML.push 1].
+  Eval compute in interpret_bfn (bfn_of_jsm [JSML.push 1; JSML.push 2; JSML.out]) [] 50.
+  
+  
+  Example bfn_of_jsm1 :
+    interpret_bfn (bfn_of_jsm [JSML.push 1]) [] 20 = Some [].
+  Proof. simpl. auto. Qed.
+    
+    
 
 End BFN.
